Extensive additions, proof attempts

Infer.v
@@ -1,9 +1,58 @@
 (* Modular network inference *)
 Require Import Coq.Init.Nat.
 Require Import Coq.Lists.List.
+Require Import Coq.Logic.FunctionalExtensionality.
+Require Import Lia.
 
-Definition iterated_and (args : list Prop) : Prop :=
-  fold_right and True args.
+Lemma map_combine :
+  forall {T1 T2 T3 T4 : Type} (l1 : list T1) (l2 : list T2) (f1 : T1 -> T3) (f2 : T2 -> T4),
+    map (fun p => (f1 (fst p), f2 (snd p))) (combine l1 l2) =
+      combine (map f1 l1) (map f2 l2).
+  Proof.
+    intros; generalize dependent l2.
+    induction l1; auto.
+    intros l2.
+    rewrite map_cons.
+    induction l2; auto.
+    simpl.
+    rewrite IHl1. reflexivity.
+Qed.
+
+Lemma combine_equal :
+  forall {T1 T2 : Type} (l1 l11 : list T1) (l2 l22 : list T2),
+    l1 = l11 -> l2 = l22 -> combine l1 l2 = combine l11 l22.
+  Proof. intros. subst. reflexivity. Qed.
+
+Lemma map_project_combine1 :
+  forall {T1 T2 T3 : Type} (l1 : list T1) (l2 : list T2) (f : T1 -> T3),
+    length l1 = length l2 ->
+    map (fun p => f (fst p)) (combine l1 l2) = map f l1.
+  Proof.
+    intros. generalize dependent l2.
+    induction l1; auto.
+    intros l2 Hlength.
+    induction l2.
+    - inversion Hlength.
+    - inversion Hlength.
+      apply IHl1 in H0. rewrite map_cons.
+      rewrite <- H0.
+      simpl. reflexivity.
+Qed.
+
+Lemma map_project_combine2 :
+  forall {T1 T2 T3 : Type} (l1 : list T1) (l2 : list T2) (f : T2 -> T3),
+    length l1 = length l2 ->
+    map (fun p => f (snd p)) (combine l1 l2) = map f l2.
+  Proof.
+    intros. generalize dependent l1.
+    induction l2.
+    - intros l1 Hlength. inversion Hlength. simpl. rewrite combine_nil. reflexivity.
+    - induction l1; intros Hlength; inversion Hlength.
+      rewrite map_cons.
+      apply IHl2 in H0.
+      rewrite <- H0.
+      simpl. reflexivity.
+Qed.
 
 Section timepiece.
   Variable S : Type.
@@ -14,79 +63,257 @@ Section timepiece.
   Variable Merge : S -> S -> S.
   Variable F : Edge -> S -> S.
 
-  Definition A := nat -> S -> Prop.
+  Definition φ := S -> Prop.
+  Definition A := nat -> φ.
 
   (* Computing a new route at a node given routes of its neighbors. *)
-  Definition updated_state (node : Node) (initial : S) (neighbors : list (Node * S)) : S :=
+  Definition updated_state (node : Node) (initial : S)
+    (neighbors : list (Node * S)) : S :=
     fold_right (fun (neighbor : (Node * S)) (st : S) =>
                   let (m, ms) := neighbor in
                   Merge st (F (m, node) ms)) initial neighbors.
 
   (* The until temporal operator. *)
-  Definition until (tau : nat) (before after : S -> Prop) : A :=
+  Definition until (tau : nat) (before after : φ) : A :=
     fun t s => if t <? tau then before s else after s.
 
+  (* The until operator, with a boolean instead of a time bound. *)
+  Definition buntil (b : bool) (before after : φ) : φ :=
+    fun s => if b then before s else after s.
+
+  Example until_example1 :
+    forall s φ, (until 0 φ (fun _ => True)) 1 s.
+  Proof. reflexivity. Qed.
+
+  Example buntil_example1 :
+    forall s φ, buntil false φ (fun _ => True) s.
+  Proof. reflexivity. Qed.
+
+  (* A record to bundle together the elements of an until temporal operator. *)
   Record Until := mkUntil
     {
       tau : nat
-    ; before : S -> Prop
-    ; after : S -> Prop
+    ; before : φ
+    ; after : φ
     }.
 
   Definition construct_until (u : Until) : A :=
     until (tau u) (before u) (after u).
 
+  (* Review of how fst/snd work with tuples of > 2 elements. *)
   Compute (snd (fst (1, 2, 3))). (* --> 2 *)
 
-  (* A helper definition for writing out the inductive condition given a particular set of states
-   and a particular time [t]. *)
-  Definition inductive_condition_aux
+  (* A helper definition for writing out the inductive condition with times
+     erased: all invariants are specified as [S -> Prop] functions. *)
+  Definition inductive_condition_untimed
+    (node : Node) (initial : S) (node_invariant : φ)
+    (neighbors : list (Node * S * φ)) :=
+    (* if every neighbor's route satisfies the invariant φ *)
+    (Forall (fun (c : Node * S * φ) => ((snd c) (snd (fst c)))) neighbors) ->
+    (* then the node's invariant holds on the updated state *)
+    (node_invariant (updated_state node initial (map (fun c => fst c) neighbors))).
+
+  (* A helper definition for writing out the inductive condition
+     given a particular set of states and a particular time [t]. *)
+  Definition inductive_condition_fixed_time
     (node : Node) (initial : S) (node_invariant : A)
-    (neighbor_constraints : list (Node * A * S)) (t : nat) :=
-    (* if all the constraints hold on the neighbors at time t... *)
-    (Forall (fun (c : Node * A * S) =>
-                          ((snd (fst c)) t (snd c))) neighbor_constraints) ->
-    (* then the constraint holds on the updated state at the node at time t + 1 *)
-      (node_invariant (1 + t)
-         (updated_state node initial (map (fun c => (fst (fst c), (snd c))) neighbor_constraints))).
+    (neighbors : list (Node * S * A)) (t : nat) :=
+    inductive_condition_untimed
+      (* apply the node's invariant at time [t + 1] *)
+      node initial (node_invariant (1 + t))
+      (* apply the neighbors' invariants at time [t] *)
+      (map (fun (c : Node * S * A) => (fst c, (snd c) t)) neighbors).
 
   (* The original inductive condition for a node [n]. *)
   Definition inductive_condition (n : Node) (initial : S) (node_invariant : A)
-                                 (neighbor_invariants : list (Node * A)) :=
+                                 (neighbors : list (Node * A)) :=
     forall (t : nat) (states : list S),
-      length states = length neighbor_invariants ->
-      inductive_condition_aux n initial node_invariant (combine neighbor_invariants states) t.
+      length states = length neighbors ->
+      inductive_condition_fixed_time
+        n initial node_invariant
+        (* squeeze the states in between the Node and the invariant *)
+        (map (fun (c : Node * A * S) => (fst (fst c), snd c, snd (fst c)))
+           (combine neighbors states)) t.
 
   Definition boolean_equals_time_bound (b : bool) (t tau : nat) :=
     b = (t <? tau).
 
+  (* Lemma relating until and buntil. *)
+  Lemma until_has_equivalent_buntil :
+    forall (b : bool) (t tau : nat) (φ1 φ2 : φ),
+      boolean_equals_time_bound b t tau ->
+      (until tau φ1 φ2) t = (buntil b φ1 φ2).
+  Proof.
+    intros.
+    extensionality s.
+    unfold boolean_equals_time_bound in H.
+    subst.
+    reflexivity.
+  Qed.
+
+  (* associate all the boolean * witness time pairs *)
+  Definition booleans_are_time_bounds (BTs : list (bool * nat)) (t : nat) : Prop :=
+    Forall (fun bt => boolean_equals_time_bound (fst bt) t (snd bt)) BTs.
+
+  Lemma untils_have_equivalent_buntils :
+    forall (neighbor_invariants : list Until) (B : list bool) (t : nat),
+      length neighbor_invariants = length B ->
+      (* if every boolean is associated with a time bound, *)
+      booleans_are_time_bounds (combine B (map tau neighbor_invariants)) t ->
+        (* then a list of invariants with explicit times *)
+        map (fun u => (construct_until u) t) neighbor_invariants =
+          (* equals a list of invariants with Bs *)
+          map (fun bu => buntil (fst bu) (before (snd bu)) (after (snd bu)))
+            (combine B neighbor_invariants).
+  Proof.
+    intros neighbor_invariants.
+    induction neighbor_invariants.
+    - intros. rewrite combine_nil. reflexivity.
+    - intros. induction B.
+      + inversion H.
+      + inversion H.
+        simpl in *.
+        inversion H0.
+        simpl in H4.
+        apply (until_has_equivalent_buntil _ _ _ (before a) (after a)) in H4.
+        unfold construct_until.
+        subst.
+        rewrite H4.
+        f_equal.
+        apply IHneighbor_invariants.
+        * assumption.
+        * assumption.
+  Qed.
+
+  (* helper to construct all the neighbors' boolean until invariants *)
+  Definition zip_boolean_untils
+    (neighbors : list (Node * Until)) (B : list bool) (states : list S)
+    : list (Node * S * φ) :=
+    map (fun (c : Node * Until * S * bool) =>
+      let (c1, nbrb) := c in
+      let (c2, st) := c1 in
+      let (nbr, u) := c2 in
+      (nbr, st, buntil nbrb (before u) (after u)))
+      (combine (combine neighbors states) B).
+
+  (* helper lemma stating that the invariants generated using zip_boolean_untils
+     are the same as the invariants generated by mapping construct_until over the
+     Untils *)
+  Lemma zip_boolean_untils_produces_equivalent_invariants :
+    forall (neighbors : list Node)
+      (neighbor_invariants : list Until)
+      (B : list bool)
+      (states : list S)
+      (t : nat),
+      (* all lists are the same length *)
+      length neighbors = length neighbor_invariants /\ length neighbor_invariants = length B /\ length B = length states ->
+      (* all booleans are associated with the taus *)
+      booleans_are_time_bounds (combine B (map tau neighbor_invariants)) t ->
+      (* zip produces a list of [Node * S * φ] which we must then relate to
+         a list of [Node * S * A] *)
+      zip_boolean_untils (combine neighbors neighbor_invariants) B states =
+        combine (combine neighbors states) (map (fun u => (construct_until u) t) neighbor_invariants).
+  Proof.
+    unfold zip_boolean_untils, booleans_are_time_bounds, boolean_equals_time_bound.
+    induction neighbors.
+    - induction neighbor_invariants; auto.
+    - induction neighbor_invariants; intros B states t [Hlen1 [Hlen2 Hlen3]] Hbtb; inversion Hlen1; inversion Hlen2; inversion Hlen3.
+      clear Hlen1 Hlen2 Hlen3.
+      induction B; inversion H1.
+      induction states; inversion H2.
+      unfold zip_boolean_untils in *.
+      simpl in *.
+      inversion Hbtb.
+      unfold buntil, construct_until, until.
+      simpl in H6.
+      subst.
+      f_equal.
+      admit.
+  Admitted.
+
   Definition boolean_inductive_condition
-    (n : Node) (initial : S) (before after : S -> Prop) (b : bool)
+    (n : Node) (initial : S) (b : bool) (u : Until)
     (neighbors : list (Node * Until)) :=
     forall (B : list bool),
       length B = length neighbors ->
-      (exists (t : nat), Forall (fun bt => let (b, tau) := bt in boolean_equals_time_bound b t tau)
-                    (combine B (map (fun nbr => tau (snd nbr)) neighbors))) ->
-                  forall (states : list S),
-                    length states = length neighbors ->
-                    (* FIXME: need to add the reference to the nbr *)
-                    (Forall (fun bs => let (b, state) := bs in
-                                    if b then (before nbr) else (after nbr)) (combine (B states) neighbors)).
-
-  Definition until_combine (T : list nat) (befores afters : list (S -> Prop)) : list A :=
-    map (fun args =>
-      match args with
-      | (tau, before, after) => until tau before after
-      end)
-        (combine (combine T befores) afters).
+      (* associate the booleans with the neighbor witness times *)
+      (exists (t : nat), booleans_are_time_bounds
+                    (combine B (map (fun nbr => tau (snd nbr)) neighbors)) t
+      /\ boolean_equals_time_bound b (1 + t) (tau u)) ->
+      (* define the inductive condition check again, but now using booleans *)
+      (forall (states : list S),
+          length states = length neighbors ->
+          inductive_condition_untimed n initial (buntil b (before u) (after u))
+              (zip_boolean_untils neighbors B states)).
 
   Lemma ind_vc_until_implies_boolean_ind_vc :
-    forall n initial tau before after neighbors neighbor_invariants B,
-      length neighbors = length B ->
+    forall (n : Node) (initial : S) (b : bool) (tau : nat) (before after : φ)
+      (neighbors : list Node) (neighbor_invariants : list Until),
       (* node_invariant = until node_tau nbefore nafter -> *)
+      length neighbors = length neighbor_invariants ->
       inductive_condition n initial (until tau before after)
-        (combine neighbors (map construct_until neighbor_invariants))
-      ->
+        (combine neighbors (map construct_until neighbor_invariants)) ->
+      boolean_inductive_condition n initial b (mkUntil tau before after)
+        (combine neighbors neighbor_invariants).
+  Proof.
+    unfold
+      inductive_condition,
+      boolean_inductive_condition,
+      inductive_condition_fixed_time,
+      booleans_are_time_bounds.
+    simpl.
+    intros n initial b tau' before' after'.
+    intros neighbors neighbor_invariants Hnbrlen Hindvc B Hblen [t [Hnbr_bounds Hn_bound]] states Hstateslen.
+    (* match up the until and buntil *)
+    apply (until_has_equivalent_buntil _ _ _ before' after') in Hn_bound.
+    rewrite <- Hn_bound.
+    rewrite (zip_boolean_untils_produces_equivalent_invariants neighbors neighbor_invariants B states t).
+    2: { repeat split; try auto.
+         - rewrite Hblen. rewrite combine_length. lia.
+         - lia. }
+    2: { unfold booleans_are_time_bounds. simpl.
+         (* rewrite <- map_combine2 in Hnbr_bounds. *)
+         rewrite map_project_combine2 in Hnbr_bounds.
+         assumption.
+         assumption.
+    }
+    rewrite combine_length in *.
+    rewrite Hnbrlen in *.
+    rewrite map_length in Hindvc.
+    rewrite PeanoNat.Nat.min_id in *.
+    apply (Hindvc t states) in Hstateslen.
+    assert (H: (map (fun c : Node * S * A => (fst c, snd c t))
+                    (map (fun c : Node * A * S => (fst (fst c), snd c, snd (fst c)))
+                       (combine
+                          (combine neighbors (map construct_until neighbor_invariants))
+                          states))) = (combine (combine neighbors states)
+       (map (fun u : Until => construct_until u t) neighbor_invariants))).
+    {
+      admit.
+    }
+    rewrite <- H.
+    assumption.
+  Admitted.
+
+  Lemma boolean_ind_vc_until_implies_ind_vc :
+    forall (n : Node) (initial : S) (b : bool) (tau : nat) (before after : φ)
+      (neighbors : list Node) (neighbor_invariants : list Until),
+      (* node_invariant = until node_tau nbefore nafter -> *)
+      length neighbors = length neighbor_invariants ->
+      boolean_inductive_condition n initial b (mkUntil tau before after)
+        (combine neighbors neighbor_invariants) ->
+      inductive_condition n initial (until tau before after)
+        (combine neighbors (map construct_until neighbor_invariants)).
+  Proof.
+  intros n initial b tau' before' after' neighbors neighbor_invariants Hnbrlen.
+  intros Hbindvc.
+  unfold inductive_condition.
+  intros t states Hlenstates.
+  unfold inductive_condition_fixed_time.
+
+  unfold zip_boolean_untils in Hbindvc.
+
+  rewrite (zip_boolean_untils_produces_equivalent_invariants neighbors neighbor_invariants B states t).
 
   (* *)
   Definition time_bounds B T :=
